A bit of reorg and remove excess output on And3.

Attempt2/Build/And3.dfy
@@ -1,4 +1,4 @@
-module Build {
+module Build.And3 {
 
   import opened Circ
   import opened Eval
@@ -7,103 +7,24 @@ module Build {
   import opened ComposeEval
   import opened Utils
   import opened MapFunction
+  import opened Equiv
+  import opened HideOutput
+  import opened Connecting
 
-  datatype AndPorts = AndPorts(
-    i_0: NP,
-    i_1: NP,
-    o: NP
-    )
-
-  function AndBehav(p: AndPorts, knowns: map<NP, bool>): (r: map<NP, bool>)
-    requires knowns.Keys == {p.i_0, p.i_1}
-    ensures r.Keys == {p.o}
-  {
-    map[p.o := knowns[p.i_0] && knowns[p.i_1]]
-  }
-
-  function InsertAndImpl(c: Circuit): (r: (Circuit, AndPorts, Equiv))
-    requires CircuitValid(c)
-    ensures CircuitValid(r.0)
-    ensures EquivValid(r.0, r.2)
-  {
-    reveal EquivValid();
-    var new_node := GetNewNode(c);
-    assert new_node !in c.NodeKind;
-    //assert forall np: NP :: np in c.PortSource.Keys ==> np.n != new_node;
-    //assert forall np: NP :: np in c.PortSource.Values ==> np.n != new_node;
-    var new_c := Circuit(
-      NodeKind := c.NodeKind[new_node := CAnd],
-      PortSource := c.PortSource
-    );
-    var i_0 := NP(new_node, INPUT_0);
-    var i_1 := NP(new_node, INPUT_1);
-    var o_0 := NP(new_node, OUTPUT_0);
-    var inputs := {i_0, i_1};
-    var outputs := {o_0};
-    var m := AndPorts(i_0, i_1, o_0);
-    var f: map<NP, bool> --> map<NP, bool> := (x: map<NP, bool>) requires x.Keys == inputs =>
-      AndBehav(m, x);
-    var e := Equiv({new_node}, inputs, outputs, f);
-    //assert ScOutputBoundary(new_c, e.sc) == {};
-    (new_c, m, e)
-  }
-
-  lemma InsertAndCorrect(c: Circuit)
-    requires CircuitValid(c)
-    ensures
-      var (new_c, m, e) := InsertAndImpl(c);
-      EquivTrue(new_c, e)
-  {
-    var (new_c, m, e) := InsertAndImpl(c);
-    var path := [m.o];
-    LengthOneNoDuplicates(path);
-    assert CircuitValid(new_c);
-    forall knowns: map<NP, bool> | knowns.Keys == e.inputs
-      ensures
-        var iv_0 := knowns[m.i_0];
-        var iv_1 := knowns[m.i_1];
-        EvaluateONP(new_c, m.o, knowns) == EvalOk(iv_0 && iv_1)
-    {
-      var iv_0 := knowns[m.i_0];
-      var iv_1 := knowns[m.i_1];
-      assert Seq.HasNoDuplicates(path);
-      assert EvaluateONP(new_c, m.o, knowns) == EvaluateONPBinary(new_c, [m.o], knowns);
-      reveal Seq.HasNoDuplicates();
-      assert EvaluateINPInner(new_c, [m.o, m.i_0], knowns) == EvalOk(iv_0);
-      assert EvaluateINPInner(new_c, [m.o, m.i_1], knowns) == EvalOk(iv_1);
-      assert EvaluateONPBinary(new_c, [m.o], knowns) == EvalOk(iv_0 && iv_1);
-      assert EvaluateONPInner(new_c, [m.o], knowns) == EvalOk(iv_0 && iv_1);
-      assert EvaluateONP(new_c, m.o, knowns) == EvalOk(iv_0 && iv_1);
-      assert Evaluate(new_c, m.o, knowns) == EvalOk(iv_0 && iv_1);
-      assert Evaluate(new_c, m.o, knowns) == EvalOk(e.f(knowns)[m.o]);
-    }
-    assert EquivTrue(new_c, e);
-  }
-
-  function InsertAnd(c: Circuit): (r: (Circuit, AndPorts, Equiv))
-    requires CircuitValid(c)
-    ensures
-      var (new_c, m, e) := r;
-      r == InsertAndImpl(c) &&
-      EquivTrue(new_c, e)
-  {
-    InsertAndCorrect(c);
-    InsertAndImpl(c)
-  }
+  import opened And
 
   datatype And3Ports = And3Ports(
     i_0: NP,
     i_1: NP,
     i_2: NP,
-    o: NP,
-    o_extra: NP
+    o: NP
     )
 
   function And3Behav(p: And3Ports, knowns: map<NP, bool>): (r: map<NP, bool>)
     requires knowns.Keys == {p.i_0, p.i_1, p.i_2}
-    ensures r.Keys == {p.o, p.o_extra}
+    ensures r.Keys == {p.o}
   {
-    map[p.o := knowns[p.i_0] && knowns[p.i_1] &&knowns[p.i_2], p.o_extra := knowns[p.i_0] && knowns[p.i_1]]
+    map[p.o := knowns[p.i_0] && knowns[p.i_1] && knowns[p.i_2]]
   }
 
   lemma And3BehavIsComposition(p1: AndPorts, p2: AndPorts, knowns: map<NP, bool>)
@@ -113,7 +34,7 @@ module Build {
     requires p2.i_0 != p2.i_1
     requires SetsNoIntersection({p1.i_0, p1.i_1, p1.o}, {p2.i_0, p2.i_1, p2.o})
     ensures 
-      var p := And3Ports(p1.i_0, p1.i_1, p2.i_0, p2.o, p1.o);
+      var p := And3Ports(p1.i_0, p1.i_1, p2.i_0, p2.o);
       var o_base := And3Behav(p, knowns);
       var input_keys_1 := {p1.i_0, p1.i_1};
       var input_keys_2 := {p2.i_0, p2.i_1};
@@ -121,9 +42,9 @@ module Build {
       var mf2 := MapFunction(input_keys_2, {p2.o}, (x: map<NP, bool>) requires x.Keys == input_keys_2=> AndBehav(p2, x));
       var connection := map[p2.i_1 := p1.o];
       var o_compose := ComposeMapFunction(mf1, mf2, connection, knowns);
-      o_base == o_compose
+      o_base == o_compose - {p1.o}
   {
-    var p := And3Ports(p1.i_0, p1.i_1, p2.i_0, p2.o, p1.o);
+    var p := And3Ports(p1.i_0, p1.i_1, p2.i_0, p2.o);
     var o_base := And3Behav(p, knowns);
     var input_keys_1 := {p1.i_0, p1.i_1};
     var input_keys_2 := {p2.i_0, p2.i_1};
@@ -131,7 +52,7 @@ module Build {
     var mf2 := MapFunction(input_keys_2, {p2.o}, (x: map<NP, bool>) requires x.Keys == input_keys_2=> AndBehav(p2, x));
     var connection := map[p2.i_1 := p1.o];
     var o_compose := ComposeMapFunction(mf1, mf2, connection, knowns);
-    assert o_base == o_compose;
+    assert o_base == o_compose - {p1.o};
   }
 
   function {:vcs_split_on_every_assert} InsertAnd3Impl(c: Circuit): (r: (Circuit, And3Ports, Equiv))
@@ -152,13 +73,15 @@ module Build {
     EquivConserved(c2, c3, e1);
     EquivConserved(c2, c3, e2);
     var e := ComposeEquiv(c3, e1, e2);
+    assert forall np: NP :: np.n in e.sc ==> np !in c.PortSource.Values;
     var combined_input_keys := ComposeEquivInputs(c3, e1, e2);
-    var ports := And3Ports(a.i_0, a.i_1, b.i_0, b.o, a.o);
+    var ports := And3Ports(a.i_0, a.i_1, b.i_0, b.o);
     var f: map<NP, bool> --> map<NP, bool> := (x: map<NP, bool>) requires x.Keys == combined_input_keys =>
       And3Behav(ports, x);
-    var new_e := SwapEquivF(c3, e, f);
-    assert EquivValid(c3, new_e);
-    (c3, ports, new_e)
+    var e_h := EquivHideOutput(c3, e, {a.o});
+    var e_s := SwapEquivF(c3, e_h, f);
+    assert EquivValid(c3, e_s);
+    (c3, ports, e_s)
   }
 
   lemma InsertAnd3CorrectHelper(c: Circuit, e1: Equiv, e2: Equiv, knowns: map<NP, bool>)
@@ -187,23 +110,28 @@ module Build {
     reveal EquivValid();
     var (c1, a, e1) := InsertAnd(c);
     var (c2, b, e2) := InsertAnd(c1);
-    var p := And3Ports(a.i_0, a.i_1, b.i_0, b.o, a.o);
+    var p := And3Ports(a.i_0, a.i_1, b.i_0, b.o);
     var c3 := Connect(c2, b.i_1, a.o);
+    ConnectPreservesSubcircuit(c2, b.i_1, a.o, e1.sc);
+    ConnectPreservesSubcircuit(c2, b.i_1, a.o, e2.sc);
     reveal ComposedValid();
+    assert forall np: NP :: np.n in e1.sc ==> np !in c.PortSource.Values;
+    assert forall np: NP :: np.n in e2.sc ==> np !in c.PortSource.Values;
     EquivConserved(c1, c2, e1);
     EquivConserved(c2, c3, e1);
     EquivConserved(c2, c3, e2);
     var e_alt := ComposeEquiv(c3, e1, e2);
     ComposeEquivCorrect(c3, e1, e2);
     assert EquivTrue(c3, e_alt);
+    var e_rem := EquivHideOutput(c3, e_alt, {a.o});
     var combined_input_keys := ComposeEquivInputs(c3, e1, e2);
     forall knowns: map<NP, bool> | knowns.Keys == combined_input_keys
-      ensures e_alt.f(knowns) == e.f(knowns)
+      ensures e_rem.f(knowns) == e.f(knowns)
     {
       And3BehavIsComposition(a, b, knowns);
-      assert e_alt.f(knowns) == ComposeEquivF(c3, e1, e2, knowns);
+      assert e_rem.f(knowns) == ComposeEquivF(c3, e1, e2, knowns) - {a.o};
       assert e.f(knowns) == And3Behav(p, knowns);
-      assert e_alt.f(knowns) == e.f(knowns);
+      assert e_rem.f(knowns) == e.f(knowns);
     }
     assert EquivTrue(c3, e);
   }
