Attempt2/Build/And.dfy
@@ -1,0 +1,100 @@
+module Build.And {
+
+  import opened Circ
+  import opened Equiv
+  import opened Eval
+
+  datatype AndPorts = AndPorts(
+    i_0: NP,
+    i_1: NP,
+    o: NP
+    )
+
+  function AndBehav(p: AndPorts, knowns: map<NP, bool>): (r: map<NP, bool>)
+    requires knowns.Keys == {p.i_0, p.i_1}
+    ensures r.Keys == {p.o}
+  {
+    map[p.o := knowns[p.i_0] && knowns[p.i_1]]
+  }
+
+  function InsertAndImpl(c: Circuit): (r: (Circuit, AndPorts, Equiv))
+    requires CircuitValid(c)
+    ensures CircuitValid(r.0)
+    ensures EquivValid(r.0, r.2)
+  {
+    reveal EquivValid();
+    var new_node := GetNewNode(c);
+    assert new_node !in c.NodeKind;
+    //assert forall np: NP :: np in c.PortSource.Keys ==> np.n != new_node;
+    //assert forall np: NP :: np in c.PortSource.Values ==> np.n != new_node;
+    var new_c := Circuit(
+      NodeKind := c.NodeKind[new_node := CAnd],
+      PortSource := c.PortSource
+    );
+    var i_0 := NP(new_node, INPUT_0);
+    var i_1 := NP(new_node, INPUT_1);
+    var o_0 := NP(new_node, OUTPUT_0);
+    var inputs := {i_0, i_1};
+    var outputs := {o_0};
+    var m := AndPorts(i_0, i_1, o_0);
+    var f: map<NP, bool> --> map<NP, bool> := (x: map<NP, bool>) requires x.Keys == inputs =>
+      AndBehav(m, x);
+    var e := Equiv({new_node}, inputs, outputs, f);
+    //assert ScOutputBoundary(new_c, e.sc) == {};
+    (new_c, m, e)
+  }
+
+  lemma InsertAndCorrect(c: Circuit)
+    requires CircuitValid(c)
+    ensures
+      var (new_c, m, e) := InsertAndImpl(c);
+      EquivTrue(new_c, e)
+  {
+    var (new_c, m, e) := InsertAndImpl(c);
+    var path := [m.o];
+    LengthOneNoDuplicates(path);
+    assert CircuitValid(new_c);
+    forall knowns: map<NP, bool> | knowns.Keys == e.inputs
+      ensures
+        var iv_0 := knowns[m.i_0];
+        var iv_1 := knowns[m.i_1];
+        EvaluateONP(new_c, m.o, knowns) == EvalOk(iv_0 && iv_1)
+    {
+      var iv_0 := knowns[m.i_0];
+      var iv_1 := knowns[m.i_1];
+      assert Seq.HasNoDuplicates(path);
+      assert EvaluateONP(new_c, m.o, knowns) == EvaluateONPBinary(new_c, [m.o], knowns);
+      reveal Seq.HasNoDuplicates();
+      assert EvaluateINPInner(new_c, [m.o, m.i_0], knowns) == EvalOk(iv_0);
+      assert EvaluateINPInner(new_c, [m.o, m.i_1], knowns) == EvalOk(iv_1);
+      assert EvaluateONPBinary(new_c, [m.o], knowns) == EvalOk(iv_0 && iv_1);
+      assert EvaluateONPInner(new_c, [m.o], knowns) == EvalOk(iv_0 && iv_1);
+      assert EvaluateONP(new_c, m.o, knowns) == EvalOk(iv_0 && iv_1);
+      assert Evaluate(new_c, m.o, knowns) == EvalOk(iv_0 && iv_1);
+      assert Evaluate(new_c, m.o, knowns) == EvalOk(e.f(knowns)[m.o]);
+    }
+    assert EquivTrue(new_c, e);
+  }
+
+  function InsertAnd(c: Circuit): (r: (Circuit, AndPorts, Equiv))
+    requires CircuitValid(c)
+    ensures
+      var (new_c, m, e) := r;
+      r == InsertAndImpl(c) &&
+      EquivTrue(new_c, e)
+  {
+    InsertAndCorrect(c);
+    InsertAndImpl(c)
+  }
+
+  lemma InsertAndScOutputBoundaryEmpty(c: Circuit)
+    requires CircuitValid(c)
+    ensures
+      var (new_c, p, e) := InsertAnd(c);
+      ScOutputBoundary(new_c, e.sc) == {}
+  {
+    var (new_c, p, e) := InsertAnd(c);
+    assert forall np: NP :: np.n in e.sc ==> np !in c.PortSource.Values;
+  }
+
+}
