Attempt2/Connecting.dfy
@@ -1,0 +1,28 @@
+module Connecting {
+
+  import opened Circ
+  import opened ConservedSubcircuit
+
+  lemma ConnectPreservesSubcircuit(c: Circuit, inp: NP, onp: NP, sc: set<CNode>)
+    requires CircuitValid(c)
+    requires ScValid(c, sc)
+    requires inp !in c.PortSource
+    requires INPValid(c, inp)
+    requires ONPValid(c, onp)
+    requires !(inp.n in sc && onp.n in sc)
+    ensures
+      var r := Connect(c, inp, onp);
+      SubcircuitConserved(c, r, sc)
+  {
+    var ca := c;
+    var cb := Connect(c, inp, onp);
+    assert (forall n :: n in sc ==> n in ca.NodeKind && n in cb.NodeKind);
+    assert (forall n :: n in sc ==> ca.NodeKind[n] == cb.NodeKind[n]);
+    assert (forall n :: n in sc ==> ca.NodeKind[n] == cb.NodeKind[n]);
+    assert (forall np: NP :: (np in ScInputBoundary(ca, sc)) == (np in ScInputBoundary(cb, sc)));
+    assert (forall np: NP :: (np !in ScInputBoundary(ca, sc)) && np.n in sc ==> (np in ca.PortSource) == (np in cb.PortSource));
+    assert (forall np: NP :: (np !in ScInputBoundary(ca, sc)) && np.n in sc && np in ca.PortSource ==> ca.PortSource[np] == cb.PortSource[np]);
+  }
+
+
+}
