Attempt2/Equiv.dfy
@@ -1,0 +1,60 @@
+module Equiv {
+
+  import opened Circ
+  import opened Utils
+  import opened MapFunction
+  import opened Eval
+
+  // An equivalence maps a subcircuit and a node in that subcircuit to a function.
+  datatype Equiv = Equiv(
+    sc: set<CNode>,
+    inputs: set<NP>,
+    outputs: set<NP>,
+    f: map<NP, bool> --> map<NP, bool>
+  )
+
+  function EtoMf(e: Equiv): (r: MapFunction)
+  {
+    MapFunction(e.inputs, e.outputs, e.f)
+  }
+
+  lemma EValidMfValid(c: Circuit, e: Equiv)
+    requires EquivValid(c, e)
+    ensures MapFunctionValid(EtoMf(e))
+  {
+    reveal EquivValid();
+  }
+
+  function SwapEquivF(c: Circuit, e: Equiv, f: map<NP, bool> --> map<NP, bool>): (r: Equiv)
+    requires EquivValid(c, e)
+    requires (forall knowns: map<NP, bool> :: (knowns.Keys == e.inputs) ==> f.requires(knowns))
+    requires (forall knowns: map<NP, bool> :: (knowns.Keys == e.inputs) ==> f(knowns).Keys == e.outputs)
+    ensures EquivValid(c, r)
+  {
+    reveal EquivValid();
+    Equiv(e.sc, e.inputs, e.outputs, f)
+  }
+
+  ghost opaque predicate EquivValid(c: Circuit, e: Equiv)
+  {
+    ScValid(c, e.sc) &&
+    (ScInputBoundary(c, e.sc) == e.inputs) &&
+    SetsNoIntersection(e.inputs, e.outputs) &&
+    (forall np :: np in e.outputs ==> (INPValid(c, np) || ONPValid(c, np)) && np.n in e.sc) &&
+    (forall knowns: map<NP, bool> :: (knowns.Keys == e.inputs) ==> e.f.requires(knowns)) &&
+    (forall knowns: map<NP, bool> :: (knowns.Keys == e.inputs) ==> e.f(knowns).Keys == e.outputs) &&
+    // But it is possible to have outputs that are not on output boundary (i.e. we plan to connect them in the future)
+    (forall np :: np in ScOutputBoundary(c, e.sc) ==> np in e.outputs)
+  }
+
+  ghost predicate EquivTrue(c: Circuit, e: Equiv)
+    requires CircuitValid(c)
+    requires EquivValid(c, e)
+  {
+    reveal EquivValid();
+    forall knowns: map<NP, bool> :: (knowns.Keys == e.inputs) ==>
+      forall np :: np in e.outputs ==>
+        Evaluate(c, np, knowns) == EvalOk(e.f(knowns)[np])
+  }
+
+}
