Attempt2/HideOutput.dfy
@@ -1,0 +1,18 @@
+module HideOutput {
+
+  import opened Circ
+  import opened Equiv
+  import opened Utils
+
+  function EquivHideOutput(c: Circuit, e: Equiv, remove: set<NP>): (r: Equiv)
+    requires CircuitValid(c)
+    requires EquivValid(c, e)
+    requires forall np :: np in remove ==> np !in ScOutputBoundary(c, e.sc)
+    ensures EquivValid(c, r)
+    ensures EquivTrue(c, e) ==> EquivTrue(c, r)
+  {
+    reveal EquivValid();
+    Equiv(e.sc, e.inputs, e.outputs - remove, (x: map<NP, bool>) requires x.Keys == e.inputs => e.f(x) - remove)
+  }
+
+}
